{
  "@context": {
    "@language": "en",
    "dct": "http://purl.org/dc/terms/",
    "owl": "http://www.w3.org/2002/07/owl#",
    "prov": "http://www.w3.org/ns/prov#",
    "rdf": "http://www.w3.org/1999/02/22-rdf-syntax-ns#",
    "rdfs": "http://www.w3.org/2000/01/rdf-schema#",
    "schema": "http://schema.org/",
    "sh": "http://www.w3.org/ns/shacl#",
    "skos": "http://www.w3.org/2004/02/skos/core#",
    "xsd": "http://www.w3.org/2001/XMLSchema#"
  },
  "@graph": [
    {
      "@id": "http://example.org/#Pancake",
      "@type": "http://example.org/#Component",
      "dct:identifier": {
        "@id": "http://www.wikidata.org/entity/Q44541"
      },
      "http://example.org/#madeFrom": {
        "@id": "http://example.org/#Batter"
      },
      "skos:altLabel": {
        "@language": "fr",
        "@value": "CrÃªpe"
      },
      "skos:closeMatch": {
        "@id": "http://www.wikidata.org/entity/Q12200"
      },
      "skos:definition": "A thin, round cake made from a batter of eggs, milk, and flour.",
      "skos:narrower": [
        {
          "@id": "http://www.wikidata.org/entity/Q815898"
        },
        {
          "@id": "http://www.wikidata.org/entity/Q899392"
        },
        {
          "@id": "http://www.wikidata.org/entity/Q1025010"
        }
      ],
      "skos:prefLabel": "Pancake"
    },
    {
      "@id": "http://example.org/#NOM_Vocab",
      "@type": "skos:ConceptScheme",
      "dct:publisher": {
        "@id": "https://derwen.ai/"
      },
      "skos:definition": "A mid-level SKOS/OWL ontology used in the `kglab` examples",
      "skos:prefLabel": "NOM Example Vocabulary"
    },
    {
      "@id": "http://example.org/#Component",
      "@type": "skos:Concept",
      "dct:identifier": {
        "@id": "http://www.wikidata.org/entity/Q746549"
      },
      "skos:altLabel": "Dish",
      "skos:definition": "A specific prepared food which is ready to eat or used in building another dish.",
      "skos:prefLabel": "Component"
    },
    {
      "@id": "http://example.org/#Mixing",
      "@type": "http://example.org/#Component",
      "skos:closeMatch": {
        "@id": "https://www.foodonline.com/solution/mixing-and-blending"
      },
      "skos:definition": "A process of combining two or more separate components to produce a certain level of homogeneity.",
      "skos:prefLabel": "Mixing"
    },
    {
      "@id": "http://example.org/#Dough",
      "@type": "http://example.org/#Component",
      "dct:identifier": {
        "@id": "http://www.wikidata.org/entity/Q178024"
      },
      "http://example.org/#usesProcess": {
        "@id": "http://example.org/#Kneading"
      },
      "skos:definition": "A flour-based paste used to prepare food.",
      "skos:prefLabel": "Dough"
    },
    {
      "@id": "http://example.org/#usesProcess",
      "rdfs:domain": {
        "@id": "http://example.org/#Component"
      },
      "rdfs:range": {
        "@id": "http://example.org/#Process"
      }
    },
    {
      "@id": "http://example.org/#madeFrom",
      "rdfs:domain": {
        "@id": "http://example.org/#Component"
      },
      "rdfs:range": {
        "@id": "http://example.org/#Component"
      }
    },
    {
      "@id": "http://example.org/#Noodle",
      "@type": "http://example.org/#Component",
      "dct:identifier": {
        "@id": "http://www.wikidata.org/entity/Q192874"
      },
      "http://example.org/#madeFrom": {
        "@id": "http://example.org/#Dough"
      },
      "skos:altLabel": "Dumpling",
      "skos:closeMatch": {
        "@id": "http://www.wikidata.org/entity/Q1854639"
      },
      "skos:definition": "A type of staple food made from some type of unleavened dough.",
      "skos:narrower": [
        {
          "@id": "http://www.wikidata.org/entity/Q20065"
        },
        {
          "@id": "http://www.wikidata.org/entity/Q178"
        }
      ],
      "skos:prefLabel": "Noodle"
    },
    {
      "@id": "http://example.org/#Batter",
      "@type": "http://example.org/#Component",
      "dct:identifier": {
        "@id": "http://www.wikidata.org/entity/Q29493"
      },
      "http://example.org/#usesProcess": {
        "@id": "http://example.org/#Mixing"
      },
      "skos:definition": "A flour-based mixture used to prepare food.",
      "skos:prefLabel": "Batter"
    },
    {
      "@id": "http://example.org/#Process",
      "@type": "skos:Concept",
      "dct:identifier": {
        "@id": "http://www.wikidata.org/entity/Q627371"
      },
      "skos:altLabel": [
        "Food Processing",
        "Cooking"
      ],
      "skos:definition": "The transformation of raw ingredients into food, or of food into other forms.",
      "skos:prefLabel": "Process"
    },
    {
      "@id": "http://example.org/#Kneading",
      "@type": "http://example.org/#Component",
      "dct:identifier": {
        "@id": "http://www.wikidata.org/entity/Q3089784"
      },
      "skos:definition": "A process in the making of bread or dough, used to mix the ingredients and add strength to the final product.",
      "skos:prefLabel": "Kneading"
    }
  ]
}