@prefix nom:  <http://example.org/#> .
@prefix dct:  <http://purl.org/dc/terms/> .
@prefix owl:  <http://www.w3.org/2002/07/owl#> .
@prefix rdf:  <http://www.w3.org/1999/02/22-rdf-syntax-ns#> .
@prefix rdfs: <http://www.w3.org/2000/01/rdf-schema#> .
@prefix skos: <http://www.w3.org/2004/02/skos/core#> .
@prefix wd:   <http://www.wikidata.org/entity/> .

nom:NOM_Vocab a skos:ConceptScheme ;
    skos:prefLabel "NOM Example Vocabulary"@en ;
    skos:definition "A mid-level SKOS/OWL ontology used in the `kglab` examples"@en ;
    dct:publisher <https://derwen.ai/>
.


nom:Process a skos:Concept ;
    skos:prefLabel "Process"@en ;
    skos:altLabel "Food Processing"@en ;
    skos:altLabel "Cooking"@en ;
    skos:definition "The transformation of raw ingredients into food, or of food into other forms."@en ;
    dct:identifier wd:Q627371
.

nom:Mixing a nom:Component ;
    skos:prefLabel "Mixing"@en ;
    skos:definition "A process of combining two or more separate components to produce a certain level of homogeneity."@en ;
    skos:closeMatch <https://www.foodonline.com/solution/mixing-and-blending> ;
.

nom:Kneading a nom:Component ;
    skos:prefLabel "Kneading"@en ;
    skos:definition "A process in the making of bread or dough, used to mix the ingredients and add strength to the final product."@en ;
    dct:identifier wd:Q3089784 ;
.

nom:usesProcess rdfs:domain nom:Component ;
  rdfs:range nom:Process ;
.


nom:Component a skos:Concept ;
    skos:prefLabel "Component"@en ;
    skos:altLabel "Dish"@en ;
    skos:definition "A specific prepared food which is ready to eat or used in building another dish."@en ;
    dct:identifier wd:Q746549
.

nom:Dough a nom:Component ;
    skos:prefLabel "Dough"@en ;
    skos:definition "A flour-based paste used to prepare food."@en ;
    dct:identifier wd:Q178024 ;
    nom:usesProcess nom:Kneading
.

nom:Batter a nom:Component ;
    skos:prefLabel "Batter"@en ;
    skos:definition "A flour-based mixture used to prepare food."@en ;
    dct:identifier wd:Q29493 ;
    nom:usesProcess nom:Mixing
.

nom:madeFrom rdfs:domain nom:Component ;
  rdfs:range nom:Component ;
.

nom:Noodle a nom:Component ;
    skos:prefLabel "Noodle"@en ;
    skos:altLabel "Dumpling"@en ;
    skos:definition "A type of staple food made from some type of unleavened dough."@en ;
    dct:identifier wd:Q192874 ;
    skos:closeMatch wd:Q1854639 ;
    skos:narrower wd:Q178, wd:Q20065 ;
    nom:madeFrom nom:Dough
.

nom:Pancake a nom:Component ;
    skos:prefLabel "Pancake"@en ;
    skos:altLabel "CrÃªpe"@fr ;
    skos:definition "A thin, round cake made from a batter of eggs, milk, and flour."@en ;
    dct:identifier wd:Q44541 ;
    skos:closeMatch wd:Q12200 ;
    skos:narrower wd:Q815898, wd:Q899392, wd:Q1025010 ;
    nom:madeFrom nom:Batter
.